internal/examples/semantics/interfaces.go
@@ -1,6 +1,5 @@
 package semantics
 
-// Interface with method set
 type squareInterface interface {
 	Square() uint64
 }
@@ -34,36 +33,38 @@ func testAssignInterface() bool {
 	return square == 9
 }
 
-func testEmptyInterface() bool {
-	var i interface{}
-	var j interface{}
+// Failing
+// func testEmptyInterface() bool {
+// 	var i interface{}
+// 	var j interface{}
 
-	return i == j
-}
+// 	return i == j
+// }
 
-func testStringInterface() bool {
-	var i interface{} = "string"
-	var j interface{} = "string"
+// Failing
+// func testStringInterface() bool {
+// 	var i interface{} = "string"
+// 	var j interface{} = "string"
 
-	return i == j
-}
+// 	return i == j
+// }
 
-func testTypeAssertionInterface() bool {
-	var i interface{} = NumStruct{3}
+// func testTypeAssertionInterface() bool {
+// 	var i interface{} = NumStruct{3}
 
-	return i.(NumStruct) == NumStruct{3}
-}
+// 	return i.(NumStruct) == NumStruct{3}
+// }
 
-func testMultipleInterface() bool {
-	s := NumStruct{
-		Number: 3,
-	}
+// func testMultipleInterface() bool {
+// 	s := NumStruct{
+// 		Number: 3,
+// 	}
 
-	square1 := measureSquare(s)
-	square2 := measureSquare(s)
+// 	square1 := measureSquare(s)
+// 	square2 := measureSquare(s)
 
-	return square1 == square2
-}
+// 	return square1 == square2
+// }
 
 type shapeInterface interface {
 	describe() string
@@ -94,136 +95,160 @@ func (p polygonStruct) sides() uint64 {
 	return p.Sides
 }
 
-func doublePointerInterfaceTest() bool {
-	s := shapeStruct{"circle"}
-	shapes := []shapeInterface{s, &s}
+// func doublePointerInterfaceTest() bool {
+// 	s := shapeStruct{"circle"}
+// 	shapes := []shapeInterface{s, &s}
 
-	s.Shape = "square"
+// 	s.Shape = "square"
 
-	return shapes[0].describe() != shapes[1].describe()
+// 	return shapes[0].describe() != shapes[1].describe()
+// }
+
+// func multipleFieldsInterfaceTest() bool {
+// 	s := polygonStruct{"triangle", 3}
+
+// 	return s.Shape == "triangle" && s.Sides == 3
+// }
+
+// type dogInterface interface {
+// 	Name() string
+// 	Speed() uint64
+// }
+
+// type catInterface interface {
+// 	Name() string
+// 	Weight() uint64
+// }
+
+// type Puppy string
+
+// func (p Puppy) Name() string {
+// 	return "Max"
+// }
+
+// func (p Puppy) Speed() uint64 {
+// 	return 1
+// }
+
+// type Kitten string
+
+// func (k Kitten) Name() string {
+// 	return "Max"
+// }
+
+// func (k Kitten) Weight() uint64 {
+// 	return 10
+// }
+
+// func sharedFunctionsInterfaceTest() bool {
+// 	var kit catInterface = Kitten("Kitten")
+// 	var pup dogInterface = Puppy("Puppy")
+
+// 	return pup.Name() == kit.Name()
+// }
+
+type bookInterface interface {
+	GetAuthor() string
 }
 
-func multipleFieldsInterfaceTest() bool {
-	s := polygonStruct{"triangle", 3}
-
-	return s.Shape == "triangle" && s.Sides == 3
+type NovelStruct struct {
+	Author string
 }
 
-type dogInterface interface {
-	Name() string
-	Speed() uint64
+func (n NovelStruct) GetAuthor() string {
+	return n.Author
 }
 
-type catInterface interface {
-	Name() string
-	Weight() uint64
+func WhichAuthor(b bookInterface) string {
+	return b.GetAuthor()
 }
 
-type Puppy string
+func interfaceMethodNoParamsTest() bool {
+	n := NovelStruct{
+		Author: "Steve",
+	}
 
-func (p Puppy) Name() string {
-	return "Max"
+	return WhichAuthor(n) == "Steve"
 }
 
-func (p Puppy) Speed() uint64 {
-	return 1
-}
+// type printInterface interface {
+// 	Assign(string)
+// 	GetTitle() string
+// }
 
-type Kitten string
+// type PaperStruct struct {
+// 	Title string
+// }
 
-func (k Kitten) Name() string {
-	return "Max"
-}
+// func (p *PaperStruct) Assign(t string) {
+// 	p.Title = t
+// }
 
-func (k Kitten) Weight() uint64 {
-	return 10
-}
+// func (p *PaperStruct) GetTitle() string {
+// 	return p.Title
+// }
 
-func sharedFunctionsInterfaceTest() bool {
-	var kit catInterface = Kitten("Kitten")
-	var pup dogInterface = Puppy("Puppy")
+// func acceptAddressInterfaceTest() bool {
+// 	var p1 PaperStruct
+// 	var p2 PaperStruct
+// 	p1.Assign("Sample Title")
+// 	p2.Assign("Sample Title")
 
-	return pup.Name() == kit.Name()
-}
+// 	var print1 printInterface
+// 	var print2 printInterface
 
-type printInterface interface {
-	Assign(string)
-	GetTitle() string
-}
+// 	print1 = &p1
+// 	print2 = &p2
 
-type PaperStruct struct {
-	Title string
-}
+// 	return print1.GetTitle() == print2.GetTitle()
+// }
 
-func (p *PaperStruct) Assign(t string) {
-	p.Title = t
-}
+// type Flower interface {
+// 	Petals() uint64
+// }
 
-func (p *PaperStruct) GetTitle() string {
-	return p.Title
-}
+// type Flora interface {
+// 	Flower
+// 	Genus() string
+// }
 
-func acceptAddressInterfaceTest() bool {
-	var p1 PaperStruct
-	var p2 PaperStruct
-	p1.Assign("Sample Title")
-	p2.Assign("Sample Title")
+// type Lily struct{}
 
-	var print1 printInterface
-	var print2 printInterface
+// func (l Lily) Petals() uint64 { return 3 }
+// func (l Lily) Genus() string  { return "Lillium" }
 
-	print1 = &p1
-	print2 = &p2
+// type Rose struct{}
 
-	return print1.GetTitle() == print2.GetTitle()
-}
+// func (r Rose) Petals() uint64 { return 12 }
+// func (r Rose) Genus() string  { return "Rosa" }
 
-type Flower interface {
-	Petals() uint64
-}
+// type Daisy struct{}
 
-type Flora interface {
-	Flower
-	Genus() string
-}
+// func (d Daisy) Petals() uint64 { return 5 }
+// func (d Daisy) Genus() string  { return "Bellis" }
 
-type Lily struct{}
+// func polymorphismInterfaceTest() bool {
+// 	l := new(Lily)
+// 	r := new(Rose)
+// 	d := new(Daisy)
+// 	f := [...]Flower{l, r, d}
 
-func (l Lily) Petals() uint64 { return 3 }
-func (l Lily) Genus() string  { return "Lillium" }
+// 	return f[0].Petals() == 3
+// }
 
-type Rose struct{}
+// func embeddingInterfaceTest() bool {
+// 	l := new(Lily)
+// 	r := new(Rose)
+// 	d := new(Daisy)
+// 	f := [...]Flora{l, r, d}
 
-func (r Rose) Petals() uint64 { return 12 }
-func (r Rose) Genus() string  { return "Rosa" }
+// 	return f[0].Petals() == 3
+// }
 
-type Daisy struct{}
-
-func (d Daisy) Petals() uint64 { return 5 }
-func (d Daisy) Genus() string  { return "Bellis" }
-
-func polymorphismInterfaceTest() bool {
-	l := new(Lily)
-	r := new(Rose)
-	d := new(Daisy)
-	f := [...]Flower{l, r, d}
-
-	return f[0].Petals() == 3
-}
-
-func embeddingInterfaceTest() bool {
-	l := new(Lily)
-	r := new(Rose)
-	d := new(Daisy)
-	f := [...]Flora{l, r, d}
-
-	return f[0].Petals() == 3
-}
-
-func downcastInterfaceTest() bool {
-	l := Lily{}
-	var f Flora = l
-	return f.Petals() == f.(Flower).Petals()
-}
+// func downcastInterfaceTest() bool {
+// 	l := Lily{}
+// 	var f Flora = l
+// 	return f.Petals() == f.(Flower).Petals()
+// }
 
 // slices, maps not supported
